@prefix rdf:     <http://www.w3.org/1999/02/22-rdf-syntax-ns#> .
@prefix owl:     <http://www.w3.org/2002/07/owl#> .
@prefix dcterms: <http://purl.org/dc/terms/> .
@prefix xsd:     <http://www.w3.org/2001/XMLSchema#> .
@prefix vann:    <http://purl.org/vocab/vann/> .
@prefix foaf:    <http://xmlns.com/foaf/0.1/> .
@prefix rdfs:    <http://www.w3.org/2000/01/rdf-schema#> .
@prefix voaf:    <http://purl.org/vocommons/voaf#> .
@prefix oa:      <http://www.w3.org/ns/oa#> .
@prefix dcat:    <http://www.w3.org/ns/dcat#> .
@prefix prov:    <http://www.w3.org/ns/prov#> .
@prefix cito:    <http://purl.org/spar/cito#> .
@prefix :        <http://www.w3.org/ns/duv#> .

######################################
### Metadata section              ####
######################################

<http://www.w3.org/ns/duv> a voaf:Vocabulary;
    dcterms:title "Dataset Usage Vocabulary";
    dcterms:description "The Dataset Usage Vocabulary (DUV) is used to describe consumer experiences, citations, and feedback about datasets from the human perspective."@en;
    vann:preferredNamespaceUri "http://www.w3.org/ns/duv";
    vann:preferredNamespacePrefix "duv";
    rdfs:isDefinedBy <http://www.w3.org/TR/vocab-dqv/> ;
    dcterms:created "2015-12-17"^^xsd:date;
    dcterms:publisher <http://www.w3.org/data#W3C>;
    dcterms:type <http://purl.org/adms/assettype/Ontology>;
    dcterms:creator [foaf:name "Bernadette Farias LÃ³scio"], [foaf:name "Eric G. Stephan"], [foaf:name "Sumit Purohit"] .


#### Classes here ####
######################

:Application a owl:Class, rdfs:Class ;
  rdfs:label "Application"@en ;
  rdfs:comment "Software that is capable of reading and processing a corresponding dataset."@en .

:Rating a owl:Class, rdfs:Class ;
  rdfs:label "Rating"@en ;
  rdfs:comment "Metric used to evaluate the dataset."@en .

:Citation a owl:Class, rdfs:Class ;
  rdfs:label "Citation"@en ;
  rdfs:comment "Citation in document that references dataset."@en ;
  rdfs:subClassOf cito:CitationsAct .

:Feedback a owl:Class, rdfs:Class ;
  rdfs:label "Feedback"@en ;
  rdfs:comment "Feedback on the dataset. Expresses whether the dataset was useful or not, for example."@en ;
  rdfs:subClassOf oa:Annotation .
 
:DatasetCorrection a owl:Class, rdfs:Class ;
  rdfs:label "Dataset Correction"@en ;
  rdfs:comment "A dataset correction suggested by user as part of a feedback."@en .

:WebThing a owl:Class, rdfs:Class ;
  rdfs:label "Web Thing"@en ;
  rdfs:comment "A Web of Things (WoT) device, sensor, or hardware on the Web that consumes a dataset."@en . 



##### Properties here #####
###########################

:developedBy a rdf:Property ;
  rdfs:label "developed by"@en ;
  rdfs:comment "Describes the agent associated with the development of an application."@en ;
  rdfs:range foaf:Agent .

:consumes a rdf:Property ;
  rdfs:label "consumes"@en ;
  rdfs:comment "A dataset being consumed by an application."@en ;
  rdfs:range dcat:Dataset .

:generates a rdf:Property ;
  rdfs:label "generates"@en ;
  rdfs:comment "Usage experience associated with the dataset being generated."@en ;
  rdfs:range dcat:Dataset ;
  rdfs:subPropertyOf prov:generated .

:cites a rdf:Property ;
  rdfs:label "cites"@en ;
  rdfs:comment "The citing entity cites the cited entity, either directly and explicitly (as in the reference list of a journal article), indirectly (e.g. by citing a more recent paper by the same group on the same topic), or implicitly (e.g. as in artistic quotations or parodies, or in cases of plagiarism)."@en ;
  rdfs:range dcat:Dataset .

:endorses a rdf:Property ;
  rdfs:label "endorses"@en ;
  rdfs:comment "Agent provided feedback providing endorsement of dataset."@en ;
  rdfs:range dcat:Dataset .

:retains a rdf:Property ;
  rdfs:label "retains"@en ;
  rdfs:comment "A feedback annotation may refer to another feedback annotation."@en ;
  rdfs:range :Feedback .

:has_rating a rdf:Property ;
  rdfs:label "has rating"@en ;
  rdfs:comment "An optional rating provided as part of feedback."@en ;
  rdfs:range :Rating .

:has_datasetCorrection a rdf:Property ;
  rdfs:label "has rating"@en ;
  rdfs:comment "An optional data correction provided as part of feedback."@en ;
  rdfs:range :DatasetCorrection .


